implement advance_head

concurrency/node-replication/Impl.i.dfy
@@ -2,17 +2,28 @@ include "InfiniteLogTokens.i.dfy"
 include "../../lib/Lang/LinearSequence.i.dfy"
 include "rwlock/Impl.i.dfy"
 include "../framework/Atomic.s.dfy"
+include "../framework/ThreadUtils.s.dfy"
+include "../framework/Ptrs.s.dfy"
 include "Runtime.s.dfy"
+include "CyclicBufferTokens.i.dfy"
 
 module Impl(nrifc: NRIfc) {
   import opened Atomics
   import opened ILT = InfiniteLogTokens(nrifc)
   import opened IL = InfiniteLogSSM(nrifc)
+  import opened CyclicBufferTokens
   import opened LinearSequence_i
   import opened LinearSequence_s
   import opened NativeTypes
   import opened RwLockImpl
   import opened Runtime
+  import opened ThreadUtils
+  import opened Ptrs
+
+  // TODO fill in reasonable constants for these
+  const BUFFER_SIZE: uint64 := 4096;
+  const GC_FROM_HEAD: uint64 := 19;
+  const WARN_THRESHOLD: uint64 := 1283748;
 
   /*
    * Anything which is allocated on a NUMA node
@@ -43,22 +54,33 @@ module Impl(nrifc: NRIfc) {
    * Central cyclic buffer stuff
    */
 
+  glinear datatype LocalTailTokens = LocalTailTokens(
+      glinear localTail: LocalTail,
+      glinear cbLocalTail: CBLocalTail)
+
   linear datatype NodeInfo = NodeInfo(
-    linear localTail: Atomic<uint64, LocalTail>
+    linear localTail: Atomic<uint64, LocalTailTokens>
   )
   {
     predicate WF(nodeId: NodeId) {
-      && (forall v, g :: atomic_inv(localTail, v, g) <==> g == LocalTail(nodeId, v as int))
+      && (forall v, g :: atomic_inv(localTail, v, g) <==>
+          g == LocalTailTokens(LocalTail(nodeId, v as int), CBLocalTail(nodeId, v as int)))
     }
   }
-  
+
   linear datatype NR = NR(
     linear ctail: Atomic<uint64, Ctail>,
+    linear head: Atomic<uint64, CBHead>,
+    linear globalTail: Atomic<uint64, CBGlobalTail>, // TODO Add the InfiniteLog's GlobalTail token
     linear node_info: lseq<NodeInfo>
   )
   {
     predicate WF() {
       && (forall v, g :: atomic_inv(ctail, v, g) <==> g == Ctail(v as int))
+      && (forall v, g :: atomic_inv(head, v, g) <==> g == CBHead(v as int))
+      && (forall v, g :: atomic_inv(globalTail, v, g) <==> g == CBGlobalTail(v as int))
+      && |node_info| == NUM_REPLICAS as int
+      && (forall nodeId | 0 <= nodeId < |node_info| :: nodeId in node_info)
       && (forall nodeId | 0 <= nodeId < |node_info| :: node_info[nodeId].WF(nodeId))
     }
   }
@@ -91,5 +113,81 @@ module Impl(nrifc: NRIfc) {
     // 2. Read localTail (loop until you read a good value)
 
     // 3. Take read-lock on replica; apply operation on replica
+  }
+
+  method advance_head(shared nr: NR, shared node: Node, op: nrifc.ReadonlyOp)
+  requires nr.WF()
+  requires node.WF()
+  decreases *
+  {
+    // https://github.com/vmware/node-replication/blob/1d92cb7c040458287bedda0017b97120fd8675a7/nr/src/log.rs#L570
+
+    var iteration: uint64 := 1;
+    var done := false;
+    while !done
+    invariant 0 <= iteration as int <= WARN_THRESHOLD as int
+    decreases *
+    {
+      var r := NUM_REPLICAS;
+      atomic_block var global_head := execute_atomic_load(nr.head) {
+        
+      }
+      atomic_block var f := execute_atomic_load(nr.globalTail) { }
+
+      glinear var advance_state_token;
+
+      atomic_block var min_local_tail :=
+          execute_atomic_load(lseq_peek(nr.node_info, 0).localTail)
+      {
+        ghost_acquire ltail;
+        advance_state_token := init_advance_head_state(ltail.cbLocalTail);
+        ghost_release ltail;
+      }
+
+      var idx: uint64 := 1;
+      while idx < r
+      invariant 0 <= idx <= r
+      invariant advance_state_token == AdvanceHeadState(idx as int, min_local_tail as int)
+      {
+        atomic_block var cur_local_tail :=
+            execute_atomic_load(lseq_peek(nr.node_info, idx).localTail)
+        {
+          ghost_acquire ltail;
+          advance_state_token := step_advance_head_state(ltail.cbLocalTail, advance_state_token);
+          ghost_release ltail;
+        }
+        if cur_local_tail < min_local_tail {
+          min_local_tail := cur_local_tail;
+        }
+        idx := idx + 1;
+      }
+
+      if min_local_tail == global_head {
+        if iteration == WARN_THRESHOLD {
+          print "Spending a long time in `advance_head`, are we starving?";
+          iteration := 0;
+        }
+        iteration := iteration + 1;
+
+        // TODO call `exec`
+
+        thread_yield();
+
+        dispose_anything(advance_state_token);
+      } else {
+        atomic_block var _ := execute_atomic_store(nr.head, min_local_tail)
+        {
+          ghost_acquire head;
+          head := finish_advance_head_state(head, advance_state_token);
+          ghost_release head;
+        }
+
+        if f < min_local_tail + BUFFER_SIZE - GC_FROM_HEAD { // TODO bounded int errors
+          done := true;
+        } else {
+          // TODO call `exec`
+        }
+      }
+    }
   }
 }
