concurrency/node-replication/CyclicBufferTokens.i.dfy
@@ -1,0 +1,40 @@
+include "../../lib/Lang/NativeTypes.s.dfy"
+
+module CyclicBufferTokens {
+  import opened NativeTypes
+
+  // Fixed number of replicas (in reference impl, this is variable)
+  const NUM_REPLICAS: uint64 := 4;
+
+  // Use 'CB' prefix to distinguish these from the corresponding state in the InfiniteLog
+  // state machine.
+
+  // TODO add 'ghost loc' to these types
+
+  datatype CBHead = CBHead(head: nat)
+
+  datatype CBLocalTail = CBLocalTail(nodeId: nat, tail: nat)
+
+  datatype CBGlobalTail = CBGlobalTail(tail: nat)
+
+  datatype AdvanceHeadState = AdvanceHeadState(idx: nat, min_tail: nat)
+
+  glinear method init_advance_head_state(gshared first_local_tail: CBLocalTail)
+  returns (glinear state': AdvanceHeadState)
+  requires first_local_tail.nodeId == 0
+  ensures state'.idx == 1
+  ensures state'.min_tail == first_local_tail.tail
+
+  glinear method step_advance_head_state(
+      gshared local_tail: CBLocalTail, glinear state: AdvanceHeadState)
+  returns (glinear state': AdvanceHeadState)
+  requires local_tail.nodeId == state.idx
+  ensures state' == AdvanceHeadState(state.idx + 1,
+      if state.min_tail < local_tail.tail then state.min_tail else local_tail.tail)
+
+  glinear method finish_advance_head_state(
+      glinear head: CBHead, glinear state: AdvanceHeadState)
+  returns (glinear head': CBHead)
+  requires state.idx == NUM_REPLICAS as int
+  ensures head' == CBHead(state.min_tail)
+}
